vera/VerilogEquivalenceCorrectness.v
@@ -37,7 +37,7 @@ Definition equivalent
   (inputs outputs : list (string * string))
   (v1 v2 : Verilog.vmodule)
   : Prop :=
-  forall (input_vals : list BV.t)
+  forall (input_vals : list XBV.t)
     (input_len_ok : length input_vals = length inputs)
     (final1 final2 : VerilogState),
     let init1 :=
@@ -76,6 +76,24 @@ Section V.
         AlwaysComb (BlockingAssign (NamedExpression 1%N "out") (NamedExpression 1%N "in"))
       ];
     |}.
+
+  Definition assign_out_twostep : vmodule :=
+    {|
+      modName := "assign_out";
+      modPorts := [
+        MkPort PortIn "in";
+        MkPort PortOut "out"
+      ];
+      modVariables := [
+        MkVariable Verilog.Scalar Verilog.Wire "in";
+        MkVariable Verilog.Scalar Verilog.Wire "v";
+        MkVariable Verilog.Scalar Verilog.Wire "out"
+      ];
+      modBody := [
+        AlwaysComb (BlockingAssign (NamedExpression 1%N "out") (NamedExpression 1%N "v"));
+        AlwaysComb (BlockingAssign (NamedExpression 1%N "v") (NamedExpression 1%N "in"))
+      ];
+    |}.
 End V.
 
 #[local] Open Scope Z_scope.
@@ -91,16 +109,42 @@ Proof.
   unfold assign_out, set_reg in eval2; simpl in eval2.
   repeat constructor.
   unfold multistep_eval, multistep in *.
-  eapply clos_trans_t1n in eval1.
-  eapply clos_trans_t1n in eval2.
-  inversion eval1 as [ ? step1 | ? ? step1_1 step1_2 ]; subst;
+  eapply clos_trans_t1n in eval1; inversion eval1 as [ ? step1 | ? ? step1_1 step1_2 ]; subst;
     repeat (unfold step in *; simp run_step exec_module_item exec_statement eval_expr in *; simpl in *);
     unfold set_reg in *; simpl in *; try solve_by_inverts 3%nat.
+  eapply clos_trans_t1n in eval2.
   inversion eval2 as [ ? step2 | ? ? step2_1 step2_2 ]; subst;
     repeat (unfold step in *; simp run_step exec_module_item exec_statement eval_expr in *; simpl in *);
     unfold set_reg in *; simpl in *; try solve_by_inverts 3%nat.
   inv step1.
   inv step2.
-  exists b. simpl.
+  eexists. simpl.
+  now rewrite StrMap.add_eq_o.
+Qed.
+
+Example assign_out_twostep_equivalent : equivalent [("in", "in")] [("out", "out")] assign_out assign_out_twostep.
+Proof.
+  unfold equivalent, match_on_regs.
+  intros * ? * [eval1 blocked1] [eval2 blocked2].
+  simpl in input_len_ok.
+  repeat (destruct input_vals; try solve [simpl in *; discriminate]).
+  simpl in *.
+  unfold assign_out, set_reg in eval1; simpl in eval1.
+  unfold assign_out, set_reg in eval2; simpl in eval2.
+  repeat constructor.
+  unfold multistep_eval, multistep in *.
+  eapply clos_trans_t1n in eval1; inversion eval1 as [ ? step1 | ? ? step1_1 step1_2 ]; subst;
+    repeat (unfold step in *; simp run_step exec_module_item exec_statement eval_expr in *; simpl in *);
+    unfold set_reg in *; simpl in *; try solve_by_inverts 3%nat.
+  inv step1.
+  eapply clos_trans_t1n in eval2; inversion eval2 as [ ? step2 | ? ? step2_1 step2_2 ]; subst;
+    repeat (unfold step in *; simp run_step exec_module_item exec_statement eval_expr in *; simpl in *);
+    unfold set_reg in *; simpl in *; try solve_by_inverts 3%nat.
+  inv step2_1.
+  inversion step2_2 as [ ? step2_2' | ? ? step2_2' step2_3 ]; subst;
+    repeat (unfold step in *; simp run_step exec_module_item exec_statement eval_expr in *; simpl in *);
+    unfold set_reg in *; simpl in *; try solve_by_inverts 3%nat.
+  inv step2_2'.
+  eexists. simpl.
   now rewrite StrMap.add_eq_o.
 Qed.
